skip_list/arrays/inv/skip_inv.v
@@ -6,11 +6,9 @@ From iris.heap_lang Require Import proofmode.
 From iris.bi Require Import updates.
 
 From SkipList.lib Require Import lock misc node_rep node_lt key_equiv.
-From SkipList.skip_list Require Import code.
-From SkipList.skip_list.inv Require Import list_equiv lazy_inv.
+From SkipList.skip_list.arrays Require Import code.
+From SkipList.skip_list.arrays.inv Require Import list_equiv lazy_inv.
 
-
-Local Open Scope Z.
 
 Module SkipListInv (Params: SKIP_LIST_PARAMS).
   Import Params.
@@ -20,9 +18,7 @@ Module SkipListInv (Params: SKIP_LIST_PARAMS).
   Section Proofs.
     Context `{!heapGS Σ, !gset_list_unionGS Σ, !lockG Σ}.
 
-    Definition levelN (lvl: Z) := nroot .@ "level" .@ lvl.
-
-    Fixpoint skip_list_equiv (lvl: Z) (head: node_rep) (S: gset Z) (q: frac) 
+    Fixpoint skip_list_equiv (lvl: nat) (head: node_rep) (S: gset Z) (q: frac) 
       (bot: bot_gname) (subs: list sub_gname) : iProp Σ :=
       match subs with
       | nil => False
@@ -31,23 +27,14 @@ Module SkipListInv (Params: SKIP_LIST_PARAMS).
         | nil =>
           ⌜ lvl = 0 ⌝
           ∗
-          is_bot_list (levelN lvl) head S q top_sub bot
-          ∗
-          ⌜ node_down head = None ⌝
+          is_bot_list lvl head S q top_sub bot
 
         | bot_sub :: _ =>
-          ∃ (d: loc) (down: node_rep),
           ⌜ lvl > 0 ⌝
           ∗
-          is_top_list (levelN lvl) head top_sub bot_sub
+          is_top_list lvl head top_sub bot_sub
           ∗
-          ⌜ node_down head = Some d ⌝
-          ∗
-          d ↦{#q} rep_to_node down
-          ∗
-          ⌜ node_key head = node_key down ⌝
-          ∗
-          skip_list_equiv (lvl - 1) down S q bot bot_subs
+          skip_list_equiv (lvl - 1) head S q bot bot_subs
         end
       end.
 
@@ -63,25 +50,24 @@ Module SkipListInv (Params: SKIP_LIST_PARAMS).
       skip_list_equiv MAX_HEIGHT head S q bot subs.
 
     
-    Lemma skip_list_equiv_inv (top_head: node_rep) (lvl: Z) (S: gset Z) (q: frac) 
+    Lemma skip_list_equiv_inv (top_head: node_rep) (lvl: nat) (S: gset Z) (q: frac) 
       (bot: bot_gname) (top_sub: sub_gname) (bot_subs: list sub_gname) :
       skip_list_equiv lvl top_head S q bot (top_sub :: bot_subs) ⊢ 
-        ∃ (P: Z → option loc → iProp Σ) (obot: option bot_gname),
-        inv (levelN lvl) (lazy_list_inv top_head top_sub obot P)
+        ∃ (P: node_rep → iProp Σ) (obot: option bot_gname),
+        inv (levelN lvl) (lazy_list_inv lvl top_head top_sub obot P)
         ∗
         skip_list_equiv lvl top_head S q bot (top_sub :: bot_subs).
     Proof.
       destruct bot_subs as [|bot_sub bot_subs].
       + iIntros "Htop". iExists from_bot_list, (Some bot).
-        iDestruct "Htop" as "(? & Hlazy & ?)".
-        iDestruct "Hlazy" as "(? & #Hinv)".
+        iDestruct "Htop" as "(? & ? & #Hinv)".
         iFrame "# ∗".
       + iIntros "Hlist". iExists (from_top_list bot_sub), None.
-        iDestruct "Hlist" as (d down) "(? & #Hinv & ?)".
-        iFrame "# ∗". iExists d, down. iFrame.
+        iDestruct "Hlist" as "(? & #Hinv & ?)".
+        iFrame "# ∗".
     Qed.
 
-    Lemma skip_list_equiv_sep (lvl: Z) (head: node_rep) (S: gset Z) (q1 q2: frac) 
+    Lemma skip_list_equiv_sep (lvl: nat) (head: node_rep) (S: gset Z) (q1 q2: frac) 
       (bot: bot_gname) (subs: list sub_gname) :
       skip_list_equiv lvl head S (q1 + q2) bot subs ⊢ 
         skip_list_equiv lvl head S q1 bot subs ∗ skip_list_equiv lvl head S q2 bot subs.
@@ -92,18 +78,15 @@ Module SkipListInv (Params: SKIP_LIST_PARAMS).
         first by iExFalso.
 
       destruct bot_subs as [|bot_sub bot_subs].
-      + iDestruct "Hlist" as "(%Hlvl & (Hown_frag & #Hinv) & %Hnone)".
+      + iDestruct "Hlist" as "(%Hlvl & Hown_frag & #Hinv)".
         iDestruct "Hown_frag" as "(Hown_frag1 & Hown_frag2)".
         by iFrame "# ∗".
-      + iDestruct "Hlist" as (d down) "(%Hlvl & #Hinv & %Hsome & Hd & %Hkey & Hmatch)".
+      + iDestruct "Hlist" as "(%Hlvl & #Hinv & Hmatch)".
         iPoseProof ("IHsubs" with "Hmatch") as "(Hlist1 & Hlist2)".
-        iDestruct "Hd" as "(Hd1 & Hd2)".
-        iSplitL "Hd1 Hlist1".
-        - iExists d, down. by iFrame "# ∗".
-        - iExists d, down. by iFrame "# ∗".
+        iSplitL "Hlist1"; by iFrame "# ∗".
     Qed.
 
-    Lemma skip_list_equiv_join (lvl: Z) (head: node_rep) (S1 S2: gset Z) (q1 q2: frac) 
+    Lemma skip_list_equiv_join (lvl: nat) (head: node_rep) (S1 S2: gset Z) (q1 q2: frac) 
       (bot: bot_gname) (subs: list sub_gname) :
       skip_list_equiv lvl head S1 q1 bot subs ∗ skip_list_equiv lvl head S2 q2 bot subs ⊢ 
         skip_list_equiv lvl head (S1 ∪ S2) (q1 + q2) bot subs.
@@ -114,21 +97,15 @@ Module SkipListInv (Params: SKIP_LIST_PARAMS).
         first by iExFalso.
 
       destruct bot_subs as [|bot_sub bot_subs].
-      + iDestruct "Hlist1" as "(%Hlvl & (Hown_frag1 & #Hinv) & %Hnone)".
-        iDestruct "Hlist2" as "(_ & (Hown_frag2 & _) & _)".
+      + iDestruct "Hlist1" as "(%Hlvl & Hown_frag1 & #Hinv)".
+        iDestruct "Hlist2" as "(_ & Hown_frag2 & _)".
         iCombine "Hown_frag1 Hown_frag2" as "Hown_frag".
         by iFrame "# ∗".
-      + iDestruct "Hlist1" as (d down) "(%Hlvl & #Hinv & %Hsome & Hd1 & %Hkey & Hmatch1)".
-        iDestruct "Hlist2" as (d' down') "(_ & _ & %Hsome' & Hd2 & _ & Hmatch2)".
-
-        assert (d = d') as <- by congruence.
-        iDestruct (mapsto_agree with "Hd1 Hd2") as %<-%rep_to_node_inj.
-        iCombine "Hd1 Hd2" as "Hd".
-
+      + iDestruct "Hlist1" as "(%Hlvl & #Hinv & Hmatch1)".
+        iDestruct "Hlist2" as "(_ & _ & Hmatch2)".
         iCombine "Hmatch1 Hmatch2" as "Hmatch".
         iPoseProof ("IHsubs" with "Hmatch") as "Hlist".
-        
-        iExists d, down. by iFrame "# ∗".
+        by iFrame "# ∗".
     Qed.
       
     Lemma is_skip_list_sep (v: val) (S: gset Z) (q1 q2: frac) 
@@ -142,9 +119,7 @@ Module SkipListInv (Params: SKIP_LIST_PARAMS).
       iDestruct "Hpt" as "(Hpt1 & Hpt2)".
       iDestruct (skip_list_equiv_sep with "Hlist") as "(Hlist1 & Hlist2)".
 
-      iSplitL "Hpt1 Hlist1".
-      + iExists h, head. by iFrame.
-      + iExists h, head. by iFrame.
+      iSplitL "Hpt1 Hlist1"; iExists h, head; by iFrame.
     Qed.      
     
     Lemma is_skip_list_join (v: val) (S1 S2: gset Z) (q1 q2: frac) 
