skip_list/lists/inv/lazy_inv.v
@@ -5,8 +5,8 @@ From iris.algebra Require Import auth frac_auth gset.
 From iris.heap_lang Require Import proofmode.
 
 From SkipList.lib Require Import lock misc node_rep node_lt key_equiv.
-From SkipList.arrays Require Import code.
-From SkipList.arrays.inv Require Import list_equiv.
+From SkipList.skip_list.lists Require Import code.
+From SkipList.skip_list.lists.inv Require Import list_equiv.
 
 
 Class gset_list_unionGS Σ := GsetGS { 
@@ -21,8 +21,11 @@ Record sub_gname := mk_sub_gname {
 }.
 
 Record bot_gname := mk_bot_gname {
-  s_frac: gname
+  s_frac: gname;
+  s_keys: gname
 }.
+
+Local Open Scope Z.
 
 Module LazyListInv (Params: SKIP_LIST_PARAMS).
   Import Params.
@@ -30,25 +33,31 @@ Module LazyListInv (Params: SKIP_LIST_PARAMS).
   Export ListEquiv.
 
   Section Proofs.
-    Context `{!heapGS Σ, !gset_list_unionGS Σ, !lockG Σ} (lvl: nat).
+    Context `{!heapGS Σ, !gset_list_unionGS Σ, !lockG Σ} (N: namespace).
 
-    Definition from_sub_list (obot: option sub_gname) (rep: node_rep) : iProp Σ := 
-      match obot with
-      | None => True
-      | Some bot => own (s_auth bot) (◯ {[ rep ]})
-                    ∗
-                    own (s_toks bot) (GSet {[ node_key rep ]})
+    Definition from_sub_list (obot: option sub_gname) (key: Z) (odown: option loc) : iProp Σ := 
+      match obot, odown with
+      | None, None => True
+      | Some bot, Some d => ∃ (down: node_rep),
+                            d ↦ rep_to_node down
+                            ∗
+                            own (s_auth bot) (◯ {[ down ]})
+                            ∗
+                            own (s_toks bot) (GSet {[ node_key down ]})
+                            ∗
+                            ⌜ key = node_key down ⌝
+      | _, _ => False
       end.
 
-    Definition from_bot_list : node_rep → iProp Σ := 
+    Definition from_bot_list : Z → option loc → iProp Σ := 
       from_sub_list None.
 
-    Definition from_top_list (bot: sub_gname) : node_rep → iProp Σ := 
+    Definition from_top_list (bot: sub_gname) : Z → option loc → iProp Σ := 
       from_sub_list (Some bot).
 
     Definition node_key_range : gset Z := Zlt_range INT_MIN INT_MAX.
 
-    Definition sub_list_inv (head: node_rep) (Γ: sub_gname) (P: node_rep → iProp Σ) 
+    Definition sub_list_inv (head: node_rep) (Γ: sub_gname) (P: Z → option loc → iProp Σ) 
       (S: gset node_rep) (Skeys: gset Z) (L: list node_rep) : iProp Σ := 
       ⌜ Permutation L (elements S) ⌝
       ∗
@@ -60,13 +69,15 @@ Module LazyListInv (Params: SKIP_LIST_PARAMS).
       ∗
       own (s_toks Γ) (GSet (node_key_range ∖ Skeys))
       ∗
-      list_equiv lvl ([head] ++ L) P.
+      list_equiv ([head] ++ L) P.
 
     Definition bot_list_inv (Γ: bot_gname) (Skeys: gset Z) : iProp Σ := 
-      own (s_frac Γ) (●F Skeys).
+      own (s_frac Γ) (●F Skeys)
+      ∗
+      own (s_keys Γ) (GSet (node_key_range ∖ Skeys)).
     
     Definition lazy_list_inv (head: node_rep) (sub: sub_gname) (obot: option bot_gname)
-      (P: node_rep → iProp Σ) : iProp Σ := 
+      (P: Z → option loc → iProp Σ) : iProp Σ := 
       ∃ (S: gset node_rep) (Skeys: gset Z) (L: list node_rep),
       sub_list_inv head sub P S Skeys L
       ∗
@@ -75,16 +86,14 @@ Module LazyListInv (Params: SKIP_LIST_PARAMS).
       | Some bot => bot_list_inv bot Skeys
       end.
 
-    Definition levelN (lvl: nat) := nroot .@ "level" .@ lvl.
-
     Definition is_top_list (head: node_rep) (top bot: sub_gname) : iProp Σ := 
-      inv (levelN lvl) (lazy_list_inv head top None (from_top_list bot)).
+      inv N (lazy_list_inv head top None (from_top_list bot)).
 
     Definition is_bot_list (head: node_rep) (Skeys: gset Z) (q: frac)
       (sub: sub_gname) (bot: bot_gname) : iProp Σ := 
       own (s_frac bot) (◯F{q} Skeys)
       ∗
-      inv (levelN lvl) (lazy_list_inv head sub (Some bot) from_bot_list).
+      inv N (lazy_list_inv head sub (Some bot) from_bot_list).
 
   End Proofs.
 End LazyListInv.
