skip_list/arrays/spec/link.v
@@ -4,9 +4,9 @@ From iris.algebra Require Import auth frac_auth gset.
 From iris.heap_lang Require Import proofmode.
 
 From SkipList.lib Require Import lock misc node_rep node_lt key_equiv.
-From SkipList.skip_list Require Import code.
-From SkipList.skip_list.inv Require Import list_equiv lazy_inv skip_inv.
-From SkipList.skip_list.spec Require Import find.
+From SkipList.skip_list.arrays Require Import code.
+From SkipList.skip_list.arrays.inv Require Import list_equiv lazy_inv skip_inv.
+From SkipList.skip_list.arrays.spec Require Import find.
 
 
 Local Open Scope Z.
@@ -17,60 +17,113 @@ Module LinkSpec (Params: SKIP_LIST_PARAMS).
   Export Find.
 
   Section Proofs.
-    Context `{!heapGS Σ, !gset_list_unionGS Σ, !lockG Σ} (N : namespace).
+    Context `{!heapGS Σ, !gset_list_unionGS Σ, !lockG Σ} (lvl: nat).
 
-    Theorem link_bot_spec (key: Z) (head pred succ: node_rep) (Skeys: gset Z) (q: frac)
-      (sub: sub_gname) (bot: bot_gname) (γ: gname) (odown: option loc) :
+    Theorem createAndLink_spec (key: Z) (head pred succ: node_rep) (Skeys: gset Z) (q: frac)
+      (sub: sub_gname) (bot: bot_gname) (s: loc) (h: nat) :
       INT_MIN < key < INT_MAX →
       {{{ 
-        is_bot_list N head Skeys q sub bot
+        is_bot_list 0 head Skeys q sub bot
         ∗
         (⌜ pred = head ⌝ ∨ own (s_auth sub) (◯ {[ pred ]}))
         ∗
         ⌜ node_key pred < key < node_key succ ⌝
         ∗
-        is_lock γ (node_lock pred) (in_lock (node_next pred))
+        node_next pred ↦{#1 / 2} #s
         ∗
-        node_next pred ↦{#1 / 2} rep_to_node succ
-        ∗
-        locked γ
-        ∗
-        from_bot_list key odown
+        inv (nodeN s) (node_inv s succ)
       }}}
-        link (rep_to_node pred) #key (oloc_to_val odown)
-      {{{ new, RET rep_to_node new;
-        is_bot_list N head (Skeys ∪ {[ key ]}) q sub bot
-        ∗ 
+        createAndLink (rep_to_node pred) #key #h
+      {{{ (n: loc) (new: node_rep), RET #n;
+        is_bot_list 0 head (Skeys ∪ {[ key ]}) q sub bot
+        ∗
         own (s_auth sub) (◯ {[ new ]})
         ∗ 
         own (s_toks sub) (GSet {[ node_key new ]})
         ∗ 
-        own (s_keys bot) (GSet {[ node_key new ]})
-        ∗ 
         ⌜ node_key new = key ⌝
+        ∗ 
+        node_next pred ↦{#1 / 2} #n
+        ∗
+        inv (nodeN n) (node_inv n new)
+        ∗ 
+        n ↦{#1 / 2 / 2} rep_to_node new
+        ∗
+        (node_next new +ₗ 1) ↦∗{#1 / 2} replicate h #()
+        ∗
+        ∃ (γ: gname), 
+          is_lock γ (node_lock new) (in_lock (node_next new) (S h))
+          ∗
+          in_lock (node_next new) (S h)
+          ∗
+          locked γ
       }}}.
     Proof.
-      iIntros (Hkey_range Φ) "(Hbot & #Hown_pred & %Hrange & #Hlock & Hpt & Hlocked & HP) HΦ".
+      iIntros (Hkey_range Φ) "(Hbot & #Hown_pred & %Hrange & Hpt & #Hinvs) HΦ".
       iDestruct "Hbot" as "(Hown_frag & #Hinv)".
 
       wp_lam. wp_pures. 
       wp_lam. wp_pures.
       wp_load. wp_let. 
-      wp_alloc l as "Hpt'". wp_let.
-      iDestruct "Hpt'" as "(Hpt' & Hpt'_dup)".
+
+      wp_alloc next as "Hnext"; first lia. wp_let.
+      assert (Z.to_nat (h + 1) = S h) as -> by lia.
+      iDestruct "Hnext" as "(Hnext' & Hnext)".
       
-      wp_apply (newlock_spec (in_lock l) with "[Hpt'_dup]").
-      { iExists succ; iFrame. }
-      iIntros (lk) "#Hlock'". iDestruct "Hlock'" as (γ') "Hlock'".
+      wp_apply (newlock_spec (in_lock next (S h)) with "[Hnext']").
+      { 
+        iExists (replicate (S h) #()); iFrame.
+        rewrite replicate_length //.
+      }
+      iIntros (lk) "#Hlock'". iDestruct "Hlock'" as (γ) "Hlock'".
 
       wp_pures.
-      set (new := (key, l, odown, lk)).
-      rewrite (fold_rep_to_node new).
+      rewrite (fold_rep_to_node (key, next, None, lk)).
+      set (new := (key, next, None, lk)).
+
+      wp_alloc n as "Hn". wp_let.
+      iDestruct "Hn" as "(Hn & Hn')".
+      iMod (inv_alloc (nodeN n) ⊤ (node_inv n new) with "Hn'") as "#Hinvn".
+      iDestruct "Hn" as "(Hn & Hn')".
+      wp_load. wp_lam. wp_pures.
+
+      wp_bind (acquire _).
+      iApply (acquire_spec with "[$]"); first done.
+      iNext; iIntros (v) "(Hin_lock & Hlocked)".
+      iDestruct "Hin_lock" as (vs) "(Hnext' & %Hlength)".
       
+      pose proof (list_split vs h 0) as Hsplit.
+      destruct Hsplit as [a Hsplit]; try lia.
+      destruct Hsplit as [vs1 Hsplit]; destruct Hsplit as [vs2 Hsplit].
+      destruct Hsplit as [Hvs Hsplit]; destruct Hsplit as [Hlength1 Hlength2].
+      destruct vs1; last inversion Hlength1.
+      simpl in Hvs; clear Hlength1.
+
+      rewrite Hvs array_cons.
+      iDestruct "Hnext'" as "(Hnext' & Hnext'2)".
+      rewrite replicate_S array_cons.
+      iDestruct "Hnext" as "(Hnext & Hreplicate)".
+
+      iDestruct (mapsto_agree with "Hnext Hnext'") as %<-.
+      iCombine "Hnext Hnext'" as "Hnext".
+
+      wp_pures. wp_store.
+      iDestruct "Hnext" as "(Hnext & Hnext')".
+
+      iCombine "Hnext' Hnext'2" as "Hnext'".
+      rewrite -array_cons.
+      iAssert (in_lock (node_next new) (S h)) 
+        with "[Hnext']" as "Hin_lock".
+      { 
+        iExists (#s :: vs2); iFrame. 
+        iPureIntro. rewrite Hvs // in Hlength.
+      }
+
       wp_bind (Store _ _).
-      iInv N as (S Skeys' L) "(Hinv_sub & Hinv_bot)" "Hclose".
+      iInv (nodeN s) as "Hs" "Hclose'"; unfold node_inv.
+      iInv (levelN 0) as (S Skeys' L) "(Hinv_sub & Hinv_bot)" "Hclose".
       iDestruct "Hinv_sub" as "(>%Hperm & >%Hsort & >%Hequiv & >Hown_auth & >Hown_toks & Hlist)".
-      iDestruct "Hinv_bot" as "(>Hown_frac & >Hown_keys)".
+      iDestruct "Hinv_bot" as ">Hown_frac"; unfold bot_list_inv.
 
       iAssert ⌜ pred = head ∨ In pred L ⌝%I
         with "[Hown_auth Hown_pred]" as %Hpred_range.
@@ -83,15 +136,20 @@ Module LinkSpec (Params: SKIP_LIST_PARAMS).
         set_solver.
       }
 
-      rewrite (list_equiv_insert head pred new succ L γ'); first last.
+      rewrite (list_equiv_insert 0 s n head pred new succ L γ (Datatypes.S h)); first last.
       { done. }
-      { auto. }
+      { done. }
       { assert (node_key new = key) as -> by auto; lia. }
       { rewrite /node_key/=; lia. }
 
-      iDestruct ("Hlist" with "[Hpt Hpt' Hlock HP]") as "Hlist".
-      { iNext; by iFrame "# ∗". }
-      iDestruct "Hlist" as (L' L1 L2) "(Hpt & >%Hsplit & >%Hsort' & >%Hperm' & Himp)".
+      rewrite ?loc_add_0.
+      iDestruct ("Hlist" with "[Hs Hpt Hnext Hn']") as "Hlist".
+      { 
+        rewrite /lfrac //= Qp_mul_1_r -Qp_div_div.
+        iNext; iFrame "# ∗". 
+        iPureIntro; lia.
+      }
+      iDestruct "Hlist" as (L' L1 L2) "(Hs & Hpt & >%Hsplit & >%Hsort' & >%Hperm' & Himp)".
 
       iDestruct (own_valid_2 with "Hown_frac Hown_frag") 
         as %HsubS%frac_auth_included_total%gset_included.
@@ -120,12 +178,11 @@ Module LinkSpec (Params: SKIP_LIST_PARAMS).
       { rewrite Zlt_range_spec; lia. }
       rewrite -gset_disj_union; last set_solver.
       iDestruct "Hown_toks" as "(Hown_toks & Hown_tok)".
-      iDestruct "Hown_keys" as "(Hown_keys & Hown_key)".
 
       wp_store.
       iDestruct "Hpt" as "(Hpt & Hpt_dup)".
       iPoseProof ("Himp" with "Hpt_dup") as "Hlist".
-      iMod ("Hclose" with "[Hlist Hown_auth Hown_toks Hown_frac Hown_keys]") as "_".
+      iMod ("Hclose" with "[Hlist Hown_auth Hown_toks Hown_frac]") as "_".
       {
         iNext; iExists (S ∪ {[ new ]}), (Skeys' ∪ {[ key ]}), L'. 
         iFrame. iSplit; last first. iSplit; first done.
@@ -154,59 +211,62 @@ Module LinkSpec (Params: SKIP_LIST_PARAMS).
           - set_solver.
       }
 
-      iModIntro. wp_pures. wp_lam. wp_pures.
-      wp_apply (release_spec with "[Hlock Hpt Hlocked]"); first done.
-      { iFrame "# ∗"; iExists new; iFrame. }
-      iIntros "_". wp_pures. 
-      iModIntro. iApply "HΦ".
-      by iFrame "# ∗".
+      iMod ("Hclose'" with "[$]") as "_".
+      iApply fupd_mask_intro_subseteq; first done.
+
+      wp_pures. iModIntro. iApply "HΦ".
+      iFrame "# ∗". iSplit; first done.
+      iExists γ. iFrame "# ∗".
     Qed.
 
-    Theorem link_top_spec (key: Z) (head pred succ: node_rep) 
-      (top bot: sub_gname) (γ: gname) (odown: option loc) :
+    Theorem link_spec (key: Z) (head pred new succ: node_rep) 
+      (top bot: sub_gname) (γ: gname) (s n: loc) (h: nat) :
       INT_MIN < key < INT_MAX →
       {{{ 
-        inv N (lazy_list_inv head top None (from_top_list bot))
+        inv (levelN lvl) (lazy_list_inv lvl head top None (from_top_list bot))
         ∗
         (⌜ pred = head ⌝ ∨ own (s_auth top) (◯ {[ pred ]}))
         ∗
         ⌜ node_key pred < key < node_key succ ⌝
         ∗
-        is_lock γ (node_lock pred) (in_lock (node_next pred))
+        (node_next pred +ₗ lvl) ↦{#1 / 2} #s
         ∗
-        node_next pred ↦{#1 / 2} rep_to_node succ
+        inv (nodeN s) (node_inv s succ)
         ∗
-        locked γ
+        inv (nodeN n) (node_inv n new)
+        ∗ 
+        n ↦{#lfrac lvl} rep_to_node new
         ∗
-        from_top_list bot key odown
+        (node_next new +ₗ lvl) ↦ #()
+        ∗
+        is_lock γ (node_lock new) (in_lock (node_next new) h)
+        ∗
+        ⌜ lvl < h ⌝
+        ∗
+        from_top_list bot new
+        ∗ 
+        ⌜ node_key new = key ⌝
       }}}
-        link (rep_to_node pred) #key (oloc_to_val odown)
-      {{{ new, RET rep_to_node new;
+        link (rep_to_node pred) #lvl #n
+      {{{ RET #();
         own (s_auth top) (◯ {[ new ]})
         ∗ 
         own (s_toks top) (GSet {[ node_key new ]})
-        ∗ 
-        ⌜ node_key new = key ⌝
+        ∗
+        (node_next pred +ₗ lvl) ↦{#1 / 2} #n
+        ∗
+        (node_next new +ₗ lvl) ↦{#1 / 2} #s
       }}}.
     Proof.
-      iIntros (Hkey_range Φ) "(#Hinv & #Hown_pred & %Hrange & #Hlock & Hpt & Hlocked & HP) HΦ".
+      iIntros (Hkey_range Φ) "(#Hinv & #Hown_pred & %Hrange & Hpt & #Hinvs & #Hinvn & Hn & Hnext & #Hlock & #Hlvl & HP & %Hkey) HΦ".
 
-      wp_lam. wp_pures. 
+      wp_lam. wp_pures. wp_lam. wp_pures.
+      wp_load. wp_let. wp_load. 
       wp_lam. wp_pures.
-      wp_load. wp_let. 
-      wp_alloc l as "Hpt'". wp_let.
-      iDestruct "Hpt'" as "(Hpt' & Hpt'_dup)".
+      wp_store. wp_pures.
       
-      wp_apply (newlock_spec (in_lock l) with "[Hpt'_dup]").
-      { iExists succ; iFrame. }
-      iIntros (lk) "#Hlock'". iDestruct "Hlock'" as (γ') "Hlock'".
-
-      wp_pures.
-      set (new := (key, l, odown, lk)).
-      rewrite (fold_rep_to_node new).
-      
-      wp_bind (Store _ _).
-      iInv N as (S Skeys' L) "(Hinv_sub & _)" "Hclose".
+      iInv (nodeN s) as "Hs" "Hclose'".
+      iInv (levelN lvl) as (S Skeys' L) "(Hinv_sub & _)" "Hclose".
       iDestruct "Hinv_sub" as "(>%Hperm & >%Hsort & >%Hequiv & >Hown_auth & >Hown_toks & Hlist)".
 
       iAssert ⌜ pred = head ∨ In pred L ⌝%I
@@ -220,25 +280,26 @@ Module LinkSpec (Params: SKIP_LIST_PARAMS).
         set_solver.
       }
 
-      rewrite (list_equiv_insert head pred new succ L γ'); first last.
+      rewrite (list_equiv_insert lvl s n head pred new succ L γ h); first last.
       { done. }
       { auto. }
       { assert (node_key new = key) as -> by auto; lia. }
-      { rewrite /node_key/=; lia. }
+      { rewrite Hkey /node_key/=; lia. }
 
-      iDestruct ("Hlist" with "[Hpt Hpt' Hlock HP]") as "Hlist".
-      { iNext; by iFrame "# ∗". }
-      iDestruct "Hlist" as (L' L1 L2) "(Hpt & >%Hsplit & >%Hsort' & >%Hperm' & Himp)".
+      iDestruct "Hnext" as "(Hnext & Hnext')".
+      iDestruct ("Hlist" with "[Hs Hpt Hnext' Hn HP]") as "Hlist".
+      { iNext; iFrame "# ∗". }
+      iDestruct "Hlist" as (L' L1 L2) "(Hs & Hpt & >%Hsplit & >%Hsort' & >%Hperm' & Himp)".
       
-      assert (key ∉ Skeys') as Hnin'.
+      assert (node_key new ∉ Skeys') as Hnin'.
       {
         intros Hfalse.
         rewrite -elem_of_elements Hequiv elem_of_list_In -Hperm in_map_iff in Hfalse.
-        destruct Hfalse as [x [Hkey Hin]].
+        destruct Hfalse as [x [Hkey' Hin]].
         
         apply (sorted_node_lt_nin L1 L2 pred succ x).
         { rewrite -Hsplit //. }
-        { rewrite Hkey; lia. }
+        { rewrite Hkey'; lia. }
         rewrite -Hsplit. apply in_or_app; right. apply in_or_app; by left.
       }
 
@@ -246,7 +307,7 @@ Module LinkSpec (Params: SKIP_LIST_PARAMS).
       { apply auth_update_alloc, (gset_local_update_union _ _ {[ new ]}). }
       assert (ε ∪ {[ new ]} = {[ new ]}) as -> by set_solver.
 
-      rewrite (gset_union_diff key); first last.
+      rewrite (gset_union_diff (node_key new)); first last.
       { done. }
       { rewrite Zlt_range_spec; lia. }
       rewrite -gset_disj_union; last set_solver.
@@ -257,11 +318,11 @@ Module LinkSpec (Params: SKIP_LIST_PARAMS).
       iPoseProof ("Himp" with "Hpt_dup") as "Hlist".
       iMod ("Hclose" with "[Hlist Hown_auth Hown_toks]") as "_".
       {
-        iNext; iExists (S ∪ {[ new ]}), (Skeys' ∪ {[ key ]}), L'. 
-        iFrame. iSplit; last first. iSplit; first done.
-        by (iPureIntro; apply key_equiv_insert_nin).
+        iNext; iExists (S ∪ {[ new ]}), (Skeys' ∪ {[ node_key new ]}), L'. 
+        iFrame. iPureIntro.
+        split; first last. split; first done.
+        by apply key_equiv_insert_nin.
         
-        iPureIntro.
         apply NoDup_Permutation.
         { 
           apply node_rep_sorted_app in Hsort'; destruct Hsort' as [_ Hsort']. 
@@ -284,12 +345,9 @@ Module LinkSpec (Params: SKIP_LIST_PARAMS).
           - set_solver.
       }
 
-      iModIntro. wp_pures. wp_lam. wp_pures.
-      wp_apply (release_spec with "[Hlock Hpt Hlocked]"); first done.
-      { iFrame "# ∗"; iExists new; iFrame. }
-      iIntros "_". wp_pures. 
-      iModIntro. iApply "HΦ". 
-      by iFrame.
+      iMod ("Hclose'" with "[$]") as "_".
+      iApply fupd_mask_intro_subseteq; first done.
+      iApply "HΦ". iFrame "# ∗". 
     Qed.
 
   End Proofs.
