skip_list/arrays/spec/new.v
@@ -2,8 +2,8 @@ From iris.algebra Require Import auth frac_auth gset.
 From iris.heap_lang Require Import proofmode.
 
 From SkipList.lib Require Import lock misc node_rep node_lt key_equiv.
-From SkipList.arrays Require Import code.
-From SkipList.arrays.inv Require Import list_equiv lazy_inv skip_inv.
+From SkipList.skip_list.arrays Require Import code.
+From SkipList.skip_list.arrays.inv Require Import list_equiv lazy_inv skip_inv.
 
 
 Module NewSpec (Params: SKIP_LIST_PARAMS).
